% --- ((x+2)^x)^(a*x) ---
\begin{align*}
f(x) &= {{\left(x+2\right)}^{\left(a{{x}^{2}}\right)}}\\
f(0) &= 1\\ 
f(1) &= {{3}^{a}}\\ 
f(3) &= {{5}^{\left(9a\right)}}\\ 
f(x^2) &= {{\left({{x}^{2}}+2\right)}^{\left(a{{x}^{4}}\right)}}\\
\end{align*}
\begin{align*}
f'(x) &= \varnothing\\
\end{align*}
% --- x^2+3*x^2 ---
\begin{align*}
f(x) &= 4{{x}^{2}}\\
f(0) &= 0\\ 
f(1) &= 4\\ 
f(3) &= 36\\ 
f(x^2) &= 4{{x}^{4}}\\
\end{align*}
\begin{align*}
f'(x) &= 8x\\
f'(0) &= 0\\ 
f'(1) &= 8\\
f'(3) &= 24\\ 
f'(x^2) &= 8{{x}^{2}}\\
\end{align*}
% --- 6*x*x+2*x+5 ---
\begin{align*}
f(x) &= 6{{x}^{2}}+2x+5\\
f(0) &= 5\\ 
f(1) &= 13\\ 
f(3) &= 65\\ 
f(x^2) &= 2{{x}^{2}}+6{{x}^{4}}+5\\
\end{align*}
\begin{align*}
f'(x) &= 12x+2\\
f'(0) &= 2\\ 
f'(1) &= 14\\
f'(3) &= 38\\ 
f'(x^2) &= 12{{x}^{2}}+2\\
\end{align*}
% --- x^2 ---
\begin{align*}
f(x) &= {{x}^{2}}\\
f(0) &= 0\\ 
f(1) &= 1\\ 
f(3) &= 9\\ 
f(x^2) &= {{x}^{4}}\\
\end{align*}
\begin{align*}
f'(x) &= 2x\\
f'(0) &= 0\\ 
f'(1) &= 2\\
f'(3) &= 6\\ 
f'(x^2) &= 2{{x}^{2}}\\
\end{align*}
% --- (2*x+5*x)^2+(7*x)^2 ---
\begin{align*}
f(x) &= 98{{x}^{2}}\\
f(0) &= 0\\ 
f(1) &= 98\\ 
f(3) &= 882\\ 
f(x^2) &= 98{{x}^{4}}\\
\end{align*}
\begin{align*}
f'(x) &= 196x\\
f'(0) &= 0\\ 
f'(1) &= 196\\
f'(3) &= 588\\ 
f'(x^2) &= 196{{x}^{2}}\\
\end{align*}
% --- (2*x+5*x)^2*(7*x)^3 ---
\begin{align*}
f(x) &= 16807{{x}^{5}}\\
f(0) &= 0\\ 
f(1) &= 16807\\ 
f(3) &= 4.0841\times 10^{6}\\ 
f(x^2) &= 16807{{x}^{10}}\\
\end{align*}
\begin{align*}
f'(x) &= 84035{{x}^{4}}\\
f'(0) &= 0\\ 
f'(1) &= 84035\\
f'(3) &= 6.80684\times 10^{6}\\ 
f'(x^2) &= 84035{{x}^{8}}\\
\end{align*}
% --- 2*x^2+(6*x+5)^2 ---
\begin{align*}
f(x) &= {{\left(6x+5\right)}^{2}}+2{{x}^{2}}\\
f(0) &= 25\\ 
f(1) &= 123\\ 
f(3) &= 547\\ 
f(x^2) &= {{\left(6{{x}^{2}}+5\right)}^{2}}+2{{x}^{4}}\\
\end{align*}
\begin{align*}
f'(x) &= 76x+60\\
f'(0) &= 60\\ 
f'(1) &= 136\\
f'(3) &= 288\\ 
f'(x^2) &= 76{{x}^{2}}+60\\
\end{align*}
% --- e^2 ---
\begin{align*}
f(x) &= {{e}^{2}}\\
f(0) &= {{e}^{2}}\\ 
f(1) &= {{e}^{2}}\\ 
f(3) &= {{e}^{2}}\\ 
f(x^2) &= {{e}^{2}}\\
\end{align*}
\begin{align*}
f'(x) &= 0\\
f'(0) &= 0\\ 
f'(1) &= 0\\
f'(3) &= 0\\ 
f'(x^2) &= 0\\
\end{align*}
% --- e^(2*x) ---
\begin{align*}
f(x) &= {{e}^{\left(2x\right)}}\\
f(0) &= 1\\ 
f(1) &= {{e}^{2}}\\ 
f(3) &= {{e}^{6}}\\ 
f(x^2) &= {{e}^{\left(2{{x}^{2}}\right)}}\\
\end{align*}
\begin{align*}
f'(x) &= 2{{e}^{\left(2x\right)}}\\
f'(0) &= 2\\ 
f'(1) &= 2{{e}^{2}}\\
f'(3) &= 2{{e}^{6}}\\ 
f'(x^2) &= 2{{e}^{\left(2{{x}^{2}}\right)}}\\
\end{align*}
% --- e^(2*x^3+x) ---
\begin{align*}
f(x) &= {{e}^{\left(2{{x}^{3}}+x\right)}}\\
f(0) &= 1\\ 
f(1) &= {{e}^{3}}\\ 
f(3) &= {{e}^{57}}\\ 
f(x^2) &= {{e}^{\left(2{{x}^{6}}+{{x}^{2}}\right)}}\\
\end{align*}
\begin{align*}
f'(x) &= (6{{x}^{2}}+1){{e}^{\left(2{{x}^{3}}+x\right)}}\\
f'(0) &= 1\\ 
f'(1) &= 7{{e}^{3}}\\
f'(3) &= 55{{e}^{57}}\\ 
f'(x^2) &= (6{{x}^{4}}+1){{e}^{\left(2{{x}^{6}}+{{x}^{2}}\right)}}\\
\end{align*}
% --- x*e^(5*x^2) ---
\begin{align*}
f(x) &= x{{e}^{\left(5{{x}^{2}}\right)}}\\
f(0) &= 0\\ 
f(1) &= {{e}^{5}}\\ 
f(3) &= 3{{e}^{45}}\\ 
f(x^2) &= {{x}^{2}}{{e}^{\left(5{{x}^{4}}\right)}}\\
\end{align*}
\begin{align*}
f'(x) &= 10{{x}^{2}}{{e}^{\left(5{{x}^{2}}\right)}}+{{e}^{\left(5{{x}^{2}}\right)}}\\
f'(0) &= 1\\ 
f'(1) &= 11{{e}^{5}}\\
f'(3) &= 91{{e}^{45}}\\ 
f'(x^2) &= 10{{x}^{4}}{{e}^{\left(5{{x}^{4}}\right)}}+{{e}^{\left(5{{x}^{4}}\right)}}\\
\end{align*}
% --- 2*x^2*y*x^2 ---
\begin{align*}
f(x) &= 2y{{x}^{4}}\\
f(0) &= 0\\ 
f(1) &= 2y\\ 
f(3) &= 162y\\ 
f(x^2) &= 2y{{x}^{8}}\\
\end{align*}
\begin{align*}
f'(x) &= 8y{{x}^{3}}\\
f'(0) &= 0\\ 
f'(1) &= 8y\\
f'(3) &= 216y\\ 
f'(x^2) &= 8y{{x}^{6}}\\
\end{align*}
% --- x^5*x*x^2 ---
\begin{align*}
f(x) &= {{x}^{8}}\\
f(0) &= 0\\ 
f(1) &= 1\\ 
f(3) &= 6561\\ 
f(x^2) &= {{x}^{16}}\\
\end{align*}
\begin{align*}
f'(x) &= 8{{x}^{7}}\\
f'(0) &= 0\\ 
f'(1) &= 8\\
f'(3) &= 17496\\ 
f'(x^2) &= 8{{x}^{14}}\\
\end{align*}
% --- ((x+2)^x)*(a*x) ---
\begin{align*}
f(x) &= ax{{\left(x+2\right)}^{x}}\\
f(0) &= 0\\ 
f(1) &= 3a\\ 
f(3) &= 375a\\ 
f(x^2) &= a{{x}^{2}}{{\left({{x}^{2}}+2\right)}^{\left({{x}^{2}}\right)}}\\
\end{align*}
\begin{align*}
f'(x) &= \varnothing\\
\end{align*}
% --- ((x+2)*x)*(a*x) ---
\begin{align*}
f(x) &= a{{x}^{2}}(x+2)\\
f(0) &= 0\\ 
f(1) &= 3a\\ 
f(3) &= 45a\\ 
f(x^2) &= a{{x}^{4}}({{x}^{2}}+2)\\
\end{align*}
\begin{align*}
f'(x) &= ax(2x+4)+a{{x}^{2}}\\
f'(0) &= 0\\ 
f'(1) &= 7a\\
f'(3) &= 39a\\ 
f'(x^2) &= a{{x}^{2}}(2{{x}^{2}}+4)+a{{x}^{4}}\\
\end{align*}
