${{\left({{\left(x+2\right)}^{x}}\right)}^{\left(ax\right)}}$ & $\rightarrow$ & \verb|((x+2)^x)^(a*x)|\\
${{x}^{2}}+3{{x}^{2}}$ & $\rightarrow$ & \verb|x^2+3*x^2|\\
$6xx+2x+5$ & $\rightarrow$ & \verb|6*x*x+2*x+5|\\
${{x}^{2}}$ & $\rightarrow$ & \verb|x^2|\\
${{\left(2x+5x\right)}^{2}}+{{\left(7x\right)}^{2}}$ & $\rightarrow$ & \verb|(2*x+5*x)^2+(7*x)^2|\\
${{\left(2x+5x\right)}^{2}}{{\left(7x\right)}^{3}}$ & $\rightarrow$ & \verb|(2*x+5*x)^2*(7*x)^3|\\
$2{{x}^{2}}+{{\left(6x+5\right)}^{2}}$ & $\rightarrow$ & \verb|2*x^2+(6*x+5)^2|\\
${{e}^{2}}$ & $\rightarrow$ & \verb|e^2|\\
${{e}^{\left(2x\right)}}$ & $\rightarrow$ & \verb|e^(2*x)|\\
${{e}^{\left(2{{x}^{3}}+x\right)}}$ & $\rightarrow$ & \verb|e^(2*x^3+x)|\\
$x{{e}^{\left(5{{x}^{2}}\right)}}$ & $\rightarrow$ & \verb|x*e^(5*x^2)|\\
$2{{x}^{2}}y{{x}^{2}}$ & $\rightarrow$ & \verb|2*x^2*y*x^2|\\
${{x}^{5}}x{{x}^{2}}$ & $\rightarrow$ & \verb|x^5*x*x^2|\\
${{\left(x+2\right)}^{x}}ax$ & $\rightarrow$ & \verb|((x+2)^x)*(a*x)|\\
$(x+2)xax$ & $\rightarrow$ & \verb|((x+2)*x)*(a*x)|\\
